Fix some top level theorems

src/DiskSecDef.v
@@ -22,7 +22,7 @@ Set Implicit Arguments.
 (***** WEAKENING FOR PAPER *****)
 (* This is a weaker version of trace security that only checks for unseals. 
  * I overloaded the definition here to match the paper. *)
-Fixpoint trace_secure pr tr :=
+(*Fixpoint trace_secure pr tr :=
   match tr with
   | nil => True
   |h::tl => match h with
@@ -83,66 +83,66 @@ Proof.
   specialize (IHtr1 _ H0).
   destruct a; intuition.
 Qed.
-
+*)
 
 (****** DISKSEC ******)
-Definition equivalent_for tag (d1 d2: rawdisk) :=
+Definition equivalent_for tag (d1 d2: rawdisk) (dm: domainmem) :=
   forall a,
     (d1 a = None /\ d2 a = None) \/
     (exists vs1 vs2,
        d1 a = Some vs1 /\ d2 a = Some vs2 /\
        Forall2 (fun tb1 tb2 => fst tb1 = fst tb2) (vsmerge vs1) (vsmerge vs2) /\
-       Forall2 (fun tb1 tb2 => fst tb1 = tag -> snd tb1 = snd tb2) (vsmerge vs1) (vsmerge vs2)).
+       Forall2 (fun tb1 tb2 => dm (fst tb1) = Some tag -> snd tb1 = snd tb2) (vsmerge vs1) (vsmerge vs2)).
 
 
-Definition blockmem_equivalent_for tag (bm1 bm2: block_mem tagged_block) :=
+Definition blockmem_equivalent_for tag (bm1 bm2: block_mem tagged_block) (dm: domainmem):=
   forall a,
     (bm1 a = None /\ bm2 a = None) \/
     (exists v1 v2,
        bm1 a = Some v1 /\ bm2 a = Some v2 /\
        fst v1 = fst v2 /\
-       (fst v1 = tag -> snd v1 = snd v2)).
+       (dm (fst v1) = Some tag -> snd v1 = snd v2)).
 
 
-Definition same_except tag (d1 d2: rawdisk) :=
+Definition same_except tag (d1 d2: rawdisk) (dm: domainmem) :=
   forall a,
     (d1 a = None /\ d2 a = None) \/
     (exists vs1 vs2,
        d1 a = Some vs1 /\ d2 a = Some vs2 /\
        Forall2 (fun tb1 tb2 => fst tb1 = fst tb2) (vsmerge vs1) (vsmerge vs2) /\
-       Forall2 (fun tb1 tb2 => fst tb1 <> tag -> snd tb1 = snd tb2) (vsmerge vs1) (vsmerge vs2)).
+       Forall2 (fun tb1 tb2 => dm (fst tb1) <> Some tag -> snd tb1 = snd tb2) (vsmerge vs1) (vsmerge vs2)).
 
-Definition blockmem_same_except tag (bm1 bm2: block_mem tagged_block) :=
+Definition blockmem_same_except tag (bm1 bm2: block_mem tagged_block) (dm: domainmem) :=
   forall a,
     (bm1 a = None /\ bm2 a = None) \/
     (exists v1 v2,
        bm1 a = Some v1 /\ bm2 a = Some v2 /\
        fst v1 = fst v2 /\
-       (fst v1 <> tag -> snd v1 = snd v2)).
+       (dm (fst v1) <> Some tag -> snd v1 = snd v2)).
 
 Axiom can_access_dec: forall pr t, {can_access pr t}+{~can_access pr t}.
 
 Lemma forall2_tag_refl:
-  forall l, Forall2 (fun tb1 tb2 : tag * block => fst tb1 = fst tb2) l l.
+  forall l, Forall2 (fun tb1 tb2 : tagged_block => fst tb1 = fst tb2) l l.
 Proof.
   induction l; simpl; intuition.
 Qed.
 
 Lemma forall2_tag_ne_refl:
-  forall l t, Forall2 (fun tb1 tb2 : tag * block => fst tb1 <> t -> snd tb1 = snd tb2) l l.
+  forall l t (dm: domainmem), Forall2 (fun tb1 tb2 : tagged_block => dm (fst tb1) <> Some t -> snd tb1 = snd tb2) l l.
 Proof.
   induction l; simpl; intuition.
 Qed.
 
 Lemma forall2_tag_eq_refl:
-  forall l t, Forall2 (fun tb1 tb2 : tag * block => fst tb1 = t -> snd tb1 = snd tb2) l l.
+  forall l t (dm: domainmem), Forall2 (fun tb1 tb2 : tagged_block => dm (fst tb1) = Some t -> snd tb1 = snd tb2) l l.
 Proof.
   induction l; simpl; intuition.
 Qed.
 
 Lemma equivalent_for_refl:
-  forall tag d,
-    equivalent_for tag d d.
+  forall tag d dm,
+    equivalent_for tag d d dm.
 Proof.
   unfold equivalent_for; intros.
   destruct (d a); eauto.
@@ -152,24 +152,25 @@ Proof.
 Qed.
 
 Lemma blockmem_equivalent_for_refl:
-  forall tag bm,
-    blockmem_equivalent_for tag bm bm.
+  forall tag bm dm,
+    blockmem_equivalent_for tag bm bm dm.
 Proof.
   unfold blockmem_equivalent_for; intros.
   destruct (bm a); intuition.
   right; exists t, t; intuition eauto.
 Qed.
 
+
 Lemma blockmem_equivalent_for_empty_mem:
-  forall pr, 
-    (forall tag, can_access pr tag -> blockmem_equivalent_for tag empty_mem empty_mem).
+  forall pr dm, 
+    (forall tag, can_access pr tag -> blockmem_equivalent_for tag empty_mem empty_mem dm).
 Proof.
   intros; apply blockmem_equivalent_for_refl.
 Qed.
 
 Lemma blockmem_same_except_refl:
-  forall tag bm,
-    blockmem_same_except tag bm bm.
+  forall tag bm dm,
+    blockmem_same_except tag bm bm dm.
 Proof.
   unfold blockmem_same_except; intros.
   destruct (bm a); eauto.
@@ -177,7 +178,7 @@ Proof.
 Qed.
     
 Lemma same_except_refl:
-  forall t d, same_except t d d.
+  forall t d dm, same_except t d d dm.
 Proof.
   unfold same_except; intros.
   destruct (d a); eauto.
@@ -187,23 +188,24 @@ Proof.
 Qed.
 
 Lemma blockmem_same_except_upd:
-  forall bm t h v1 v2,
-    blockmem_same_except t (upd bm h (t, v1)) (upd bm h (t, v2)).
+  forall bm t h v1 v2 dm a,
+    dm a = Some t ->
+    blockmem_same_except t (upd bm h (a, v1)) (upd bm h (a, v2)) dm.
 Proof.
   unfold blockmem_same_except; intros.
-  destruct (handle_eq_dec h a); subst.
+  destruct (handle_eq_dec h a0); subst.
   repeat rewrite upd_eq; eauto.
   right; repeat eexists; intuition eauto.
   repeat rewrite upd_ne; eauto.
-  destruct (bm a); eauto.
+  destruct (bm a0); eauto.
   right; repeat eexists; intuition eauto.
 Qed.
 
 Theorem same_except_to_equivalent_for:
-  forall t1 t2 d1 d2,
-    same_except t1 d1 d2 ->
+  forall t1 t2 d1 d2 dm,
+    same_except t1 d1 d2 dm ->
     t1 <> t2 ->
-    equivalent_for t2 d1 d2.
+    equivalent_for t2 d1 d2 dm.
 Proof.
   unfold equivalent_for, same_except; intros.
   specialize (H a); split_ors; cleanup; eauto.
@@ -213,28 +215,31 @@ Proof.
   eapply forall_forall2; auto.
   eapply Forall_impl; eauto.
   simpl; intros; apply H4; subst; eauto.
+  unfold not; intros; cleanup; eauto.
 Qed.
 
 Theorem blockmem_same_except_to_equivalent_for:
-  forall t1 t2 d1 d2,
-    blockmem_same_except t1 d1 d2 ->
+  forall t1 t2 d1 d2 dm,
+    blockmem_same_except t1 d1 d2 dm ->
     t1 <> t2 ->
-    blockmem_equivalent_for t2 d1 d2.
+    blockmem_equivalent_for t2 d1 d2 dm.
 Proof.
   unfold blockmem_equivalent_for, blockmem_same_except; intros.
   specialize (H a); split_ors; cleanup; eauto.
   right; repeat eexists; eauto.
   intros; subst; eauto.
+  apply H3; unfold not; intros; cleanup; eauto.
 Qed.
 
 
   Lemma blockmem_same_except_upd_same:
-    forall t bm bm' h b b0,
-      blockmem_same_except t bm bm' ->
-      blockmem_same_except t (upd bm h (t, b)) (upd bm' h (t, b0)).
+    forall t bm bm' h b b0 a dm,
+      dm a = Some t ->
+      blockmem_same_except t bm bm' dm ->
+      blockmem_same_except t (upd bm h (a, b)) (upd bm' h (a, b0)) dm.
   Proof.
     unfold blockmem_same_except; intros.
-    destruct (handle_eq_dec h a); subst.
+    destruct (handle_eq_dec h a0); subst.
     repeat rewrite upd_eq; eauto.
     right.
     simpl in *; do 2 eexists; intuition eauto.
@@ -243,9 +248,9 @@ Qed.
   Qed.
 
   Lemma blockmem_same_except_upd_eq:
-    forall t bm bm' h v,
-      blockmem_same_except t bm bm' ->
-      blockmem_same_except t (upd bm h v) (upd bm' h v).
+    forall t bm bm' h v dm,
+      blockmem_same_except t bm bm' dm ->
+      blockmem_same_except t (upd bm h v) (upd bm' h v) dm.
   Proof.
     unfold blockmem_same_except; intros.
     destruct (handle_eq_dec h a); subst.
@@ -257,13 +262,14 @@ Qed.
 
 
   Lemma same_except_upd_same:
-    forall t d d' n b b0 b1 b2 t2 l l0,
-      same_except t d d' ->
-      Forall2 (fun tb1 tb2 => fst tb1 <> t -> snd tb1 = snd tb2)
+    forall t d d' n b b0 b1 b2 t2 l l0 x dm,
+      dm x = Some t ->
+      same_except t d d' dm ->
+      Forall2 (fun tb1 tb2 => dm (fst tb1) <> Some t -> snd tb1 = snd tb2)
               (vsmerge (t2, b1, l)) (vsmerge (t2, b2, l0)) ->
       Forall2 (fun tb1 tb2 => fst tb1 = fst tb2) l l0 ->
-      same_except t (upd d n (t, b, vsmerge (t2, b1, l)))
-                  (upd d' n (t, b0, vsmerge (t2, b2, l0))).
+      same_except t (upd d n (x, b, vsmerge (t2, b1, l)))
+                  (upd d' n (x, b0, vsmerge (t2, b2, l0))) dm.
   Proof.
     unfold same_except; intros.
     destruct (addr_eq_dec n a); subst.
@@ -277,13 +283,13 @@ Qed.
 
 
   Lemma same_except_upd_eq:
-    forall t d d' n b b1 b2 t1 t2 l l0,
-      same_except t d d' ->
-      Forall2 (fun tb1 tb2 => fst tb1 <> t -> snd tb1 = snd tb2)
+    forall t d d' n b b1 b2 t1 t2 l l0 dm,
+      same_except t d d' dm ->
+      Forall2 (fun tb1 tb2 => dm (fst tb1) <> Some t -> snd tb1 = snd tb2)
               (vsmerge (t2, b1, l)) (vsmerge (t2, b2, l0)) ->
       Forall2 (fun tb1 tb2 => fst tb1 = fst tb2) l l0 ->
       same_except t (upd d n (t1, b, vsmerge (t2, b1, l)))
-                  (upd d' n (t1, b, vsmerge (t2, b2, l0))).
+                  (upd d' n (t1, b, vsmerge (t2, b2, l0))) dm.
   Proof.
     unfold same_except; intros.
     destruct (addr_eq_dec n a); subst.
@@ -296,9 +302,9 @@ Qed.
   Qed.
 
   Lemma same_except_sync_mem:
-    forall t d d',
-      same_except t d d' ->
-      same_except t (sync_mem d) (sync_mem d').
+    forall t d d' dm,
+      same_except t d d' dm ->
+      same_except t (sync_mem d) (sync_mem d') dm.
   Proof.
     unfold sync_mem, same_except; intros.
     specialize (H a); split_ors; cleanup; eauto.
@@ -358,11 +364,11 @@ Qed.
 
 
 Lemma possible_crash_equivalent:
-  forall d1 cd1 d2 pr,
-    (forall tag, can_access pr tag -> equivalent_for tag d1 d2) ->
+  forall d1 cd1 d2 pr dm,
+    (forall tag, can_access pr tag -> equivalent_for tag d1 d2 dm) ->
     possible_crash d1 cd1 ->
     exists cd2, possible_crash d2 cd2 /\
-    (forall tag, can_access pr tag -> equivalent_for tag cd1 cd2).
+    (forall tag, can_access pr tag -> equivalent_for tag cd1 cd2 dm).
 Proof.
   unfold equivalent_for, possible_crash; intros.
   exists(fun i => match cd1 i with
@@ -423,11 +429,11 @@ Proof.
 Qed.
 
 Lemma possible_crash_same_except:
-  forall tag d1 cd1 d2,
-    same_except tag d1 d2 ->
+  forall tag d1 cd1 d2 dm,
+    same_except tag d1 d2 dm ->
     possible_crash d1 cd1 ->
     exists cd2, possible_crash d2 cd2 /\
-    same_except tag cd1 cd2.
+    same_except tag cd1 cd2 dm.
 Proof.
   unfold same_except, possible_crash; intros.
   exists(fun i => match cd1 i with
