src/DiskSecAttacker.v
@@ -31,7 +31,6 @@ Ltac rewriteall :=
   | [H: ?x = ?y, H0: ?y = ?x |- _ ] => clear H0; repeat rewriteall
   | [H: ?x = _, H0: ?x = _ |- _ ] => rewrite H in H0; repeat rewriteall
   | [H: ?x = _, H0: _ = ?x |- _ ] => rewrite H in H0; repeat rewriteall
-  (*| [H: ?x = _ |- context [?x] ] => rewrite H; repeat rewriteall *)
   end.
 
 
@@ -43,25 +42,25 @@ Ltac cleanup:= try split_match; try logic_clean; subst; try rewriteall;
 Theorem exec_equivalent_finished:
   forall T (p: prog T) pr tr d1 d2 bm1 bm2 hm d1' bm1' hm' (r: T),
     exec pr d1 bm1 hm p (Finished d1' bm1' hm' r) tr ->
-    (forall tag, can_access pr tag -> equivalent_for tag d1 d2) ->
-    (forall tag, can_access pr tag -> blockmem_equivalent_for tag bm1 bm2) ->
+    (forall tag, can_access pr tag -> equivalent_for tag d1 d2 hm) ->
+    (forall tag, can_access pr tag -> blockmem_equivalent_for tag bm1 bm2 hm) ->
     trace_secure pr tr ->
     exists d2' bm2', exec pr d2 bm2 hm p (Finished d2' bm2' hm' r) tr /\
-    (forall tag, can_access pr tag -> equivalent_for tag d1' d2') /\
-    (forall tag, can_access pr tag -> blockmem_equivalent_for tag bm1' bm2').
+    (forall tag, can_access pr tag -> equivalent_for tag d1' d2' hm') /\
+    (forall tag, can_access pr tag -> blockmem_equivalent_for tag bm1' bm2' hm').
 Proof.
   induction p; intros;  
   inv_exec_perm; cleanup; simpl in *;
   try solve [repeat eexists; [econstructor; eauto|eauto|eauto] ].
   { (** Read **)
-    destruct tb.
+    destruct bs.
     specialize H1 with (1:= can_access_public pr) as Hx;
     specialize (Hx r); intuition; cleanup; try congruence.
     specialize H0 with (1:= can_access_public pr) as Hx;
     specialize (Hx n); intuition; cleanup; try congruence.
     destruct x0, t0.
     unfold vsmerge in *; simpl in *.
-    inversion H5; inversion H6; simpl in *; subst.
+    repeat (denote (Forall2 _ (_::_)(_::_)) as Hf; inversion Hf; clear Hf; subst).
     do 2 eexists; split.
     econstructor; eauto.
     split; eauto.
@@ -78,13 +77,14 @@ Proof.
     specialize H0 with (1:= H) as Hx;
     specialize (Hx n); intuition; cleanup; try congruence.
     unfold vsmerge in *; simpl in *.
-    inversion H10; inversion H12; simpl in *; subst.
+    repeat (denote (Forall2 _ (_::_)(_::_)) as Hf; inversion Hf; clear Hf; subst).
     eauto.
     repeat rewrite Mem.upd_ne; eauto.
     eapply H1; eauto.
   }
   { (** Write **)
-    destruct tb, tbs, t0.
+    destruct b, bs, t; simpl in *.
+    destruct (hm' n0) eqn: D.    
     destruct (can_access_dec pr t).
     { (** can access **)
       specialize H0 with (1:= can_access_public pr) as Hx;
@@ -120,7 +120,7 @@ Proof.
       econstructor; eauto.
       split; eauto.
       unfold equivalent_for; intros.
-      destruct (tag_dec t2 tag); subst; intuition.
+      destruct (tag_dec t tag); subst; intuition.
       specialize H0 with (1:= H) as Hx;
       specialize (Hx n); destruct Hx; cleanup; try congruence.
       destruct (addr_eq_dec a n); subst.
@@ -133,7 +133,34 @@ Proof.
       unfold vsmerge in *; simpl in *; eauto.
       unfold vsmerge in *; simpl in *; eauto.
       econstructor.
-      simpl; intros; intuition.
+      simpl; intros; cleanup; intuition.
+      eauto.
+      repeat rewrite Mem.upd_ne; eauto.
+      eapply H0; eauto.
+    }
+    { (** inconsistent **)
+      specialize H0 with (1:= can_access_public pr) as Hx;
+      specialize (Hx n); intuition; cleanup; try congruence.
+      specialize H1 with (1:= can_access_public pr) as Hx;
+      specialize (Hx h); intuition; cleanup; try congruence.
+      destruct x0, x1; simpl in *; cleanup.
+      do 2 eexists; split.
+      econstructor; eauto.
+      split; eauto.
+      unfold equivalent_for; intros.
+      specialize H0 with (1:= H) as Hx;
+      specialize (Hx n); destruct Hx; cleanup; try congruence.
+      destruct (addr_eq_dec a n); subst.
+      right.
+      repeat rewrite Mem.upd_eq; eauto.
+      do 2 eexists; eauto.
+      split; eauto.
+      split; eauto.
+      split.
+      unfold vsmerge in *; simpl in *; eauto.
+      unfold vsmerge in *; simpl in *; eauto.
+      econstructor.
+      simpl; intros; congruence.
       eauto.
       repeat rewrite Mem.upd_ne; eauto.
       eapply H0; eauto.
@@ -155,7 +182,7 @@ Proof.
   }
   { (** Unseal **)
     intuition.
-    destruct tb; simpl in *.
+    destruct b; simpl in *.
     specialize H1 with (1:= H) as Hx;
     specialize (Hx h); intuition; cleanup; try congruence.
     simpl in *; intuition; subst.
@@ -169,15 +196,78 @@ Proof.
     specialize H0 with (1:= H) as Hx.
     unfold sync_mem.
     specialize (Hx a); intuition; cleanup; eauto.
-    rewrite H4, H5; eauto.
-    rewrite H3, H4; eauto.
+    repeat match goal with
+           | [H: ?x = _ |- context [?x] ] => rewrite H
+           end; eauto.
+    repeat match goal with
+           | [H: ?x = _ |- context [?x] ] => rewrite H
+           end; eauto.
     destruct x, x0.
-    right; repeat eexists; eauto.
     unfold vsmerge in *; simpl in *; eauto.
-    inversion H5; subst.
-    econstructor; eauto.
-    unfold vsmerge in *; simpl in *; eauto.
-    inversion H6; subst; auto.
+    repeat (denote (Forall2 _ (_::_)(_::_)) as Hf; inversion Hf; clear Hf; subst).
+    right; repeat eexists; simpl; eauto.    
+  }
+  { (** ChDom **)
+    cleanup.
+    specialize H0 with (1:= H) as Hdt'.
+    specialize H1 with (1:= H) as Hbt'.
+    repeat eexists; [econstructor; eauto| |eauto].
+    {
+      unfold equivalent_for in *; intros.
+      specialize (Hdt' a); intuition; cleanup; eauto.
+      specialize H0 with (1:= H3) as Hx.
+      specialize (Hx a); intuition; cleanup; eauto.
+      repeat match goal with
+             | [H: ?x = _ |- context [?x] ] => rewrite H
+             end; eauto.
+      destruct x1, x2.
+      right; repeat eexists; eauto.
+      unfold vsmerge in *; simpl in *; eauto.
+      repeat (denote (Forall2 _ (_::_)(_::_)) as Hf; inversion Hf; clear Hf; subst).
+      destruct (addr_eq_dec n (fst t0)); subst.
+      - econstructor; eauto.
+        eapply forall_forall2.
+        rewrite Forall_forall; intros.
+        destruct (addr_eq_dec (fst t0) (fst (fst x))); subst.
+        + cleanup.
+          rewrite Mem.upd_eq in H7; eauto.
+          cleanup.
+          eapply forall2_forall in H17; rewrite Forall_forall in H17; eauto.
+          eapply H17; eauto.
+          setoid_rewrite <- H11; eauto.
+        + rewrite Mem.upd_ne in H7; eauto.
+          cleanup.
+          eapply forall2_forall in H15; rewrite Forall_forall in H15; eauto.
+        + eapply forall2_length; eauto.
+      - cleanup.
+        econstructor; eauto.
+        rewrite Mem.upd_ne; eauto.
+        eapply forall_forall2.
+        rewrite Forall_forall; intros.
+        destruct (addr_eq_dec n (fst (fst x))); subst.
+        + rewrite Mem.upd_eq in H7; eauto.
+          cleanup.
+          eapply forall2_forall in H17; rewrite Forall_forall in H17; eauto.
+        + rewrite Mem.upd_ne in H7; eauto.
+          cleanup.
+          eapply forall2_forall in H15; rewrite Forall_forall in H15; eauto.
+        + eapply forall2_length; eauto.
+    }
+    {
+      unfold blockmem_equivalent_for in *; intros.
+      specialize (Hbt' a); intuition; cleanup; eauto.
+      specialize H1 with (1:= H3) as Hx.
+      specialize (Hx a); intuition; cleanup; eauto.
+      repeat match goal with
+             | [H: ?x = _ |- context [?x] ] => rewrite H
+             end; eauto.
+      destruct x1, x2.
+      right; repeat eexists; eauto.
+      simpl in *; eauto.
+      destruct (addr_eq_dec n n0); subst.
+      rewrite Mem.upd_eq; eauto.
+      rewrite Mem.upd_ne; eauto.
+    }
   }
   { (** Bind **)
     apply trace_secure_app_split in H3; cleanup.
@@ -185,18 +275,23 @@ Proof.
     specialize H with (1:=H4)(2:=H7)(3:=H8)(4:=H3); cleanup.
     repeat eexists; [econstructor; eauto| |]; eauto.
   }
+
+  Unshelve.
+  all: try exact addr; eauto.
+  all: try exact nil.
+  all: try exact eq.
 Qed.
 
 
 Theorem exec_equivalent_crashed:
   forall T (p: prog T) pr tr d1 d2 bm1 bm2 hm d1' bm1' hm',
     exec pr d1 bm1 hm p (Crashed d1' bm1' hm') tr ->
-    (forall tag, can_access pr tag -> equivalent_for tag d1 d2) ->
-    (forall tag, can_access pr tag -> blockmem_equivalent_for tag bm1 bm2) ->
+    (forall tag, can_access pr tag -> equivalent_for tag d1 d2 hm) ->
+    (forall tag, can_access pr tag -> blockmem_equivalent_for tag bm1 bm2 hm) ->
     trace_secure pr tr ->
     exists d2' bm2', exec pr d2 bm2 hm p (Crashed d2' bm2' hm') tr /\
-    (forall tag, can_access pr tag -> equivalent_for tag d1' d2') /\
-    (forall tag, can_access pr tag -> blockmem_equivalent_for tag bm1' bm2').
+    (forall tag, can_access pr tag -> equivalent_for tag d1' d2' hm') /\
+    (forall tag, can_access pr tag -> blockmem_equivalent_for tag bm1' bm2' hm').
 Proof.
   induction p; intros;  
   inv_exec_perm; cleanup; simpl in *;
@@ -221,115 +316,91 @@ Proof.
   }
 Qed.
 
-
 Theorem exec_equivalent_failed:
-  forall T (p: prog T) pr tr d1 d2 bm1 bm2 hm d1' bm1' hm',
-    exec pr d1 bm1 hm p (Failed d1' bm1' hm') tr ->
-    (forall tag, can_access pr tag -> equivalent_for tag d1 d2) ->
-    (forall tag, can_access pr tag -> blockmem_equivalent_for tag bm1 bm2) ->
+  forall T (p: prog T) pr tr d1 d2 bm1 bm2 hm,
+    exec pr d1 bm1 hm p Failed tr ->
+    (forall tag, can_access pr tag -> equivalent_for tag d1 d2 hm) ->
+    (forall tag, can_access pr tag -> blockmem_equivalent_for tag bm1 bm2 hm) ->
     trace_secure pr tr ->
-    exists d2' bm2', exec pr d2 bm2 hm p (Failed d2' bm2' hm') tr /\
-    (forall tag, can_access pr tag -> equivalent_for tag d1' d2') /\
-    (forall tag, can_access pr tag -> blockmem_equivalent_for tag bm1' bm2').
+    exec pr d2 bm2 hm p Failed tr.
 Proof.
   induction p; intros;  
-  inv_exec_perm; cleanup; simpl in *;
-  try solve [repeat eexists; [econstructor; eauto|eauto|eauto] ].
+    inv_exec_perm; cleanup; simpl in *;
+  try solve [econstructor; eauto].
   { (** Read **)
     specialize H0 with (1:= can_access_public pr) as Hx;
-    specialize (Hx n); intuition; cleanup; try congruence.
-    do 2 eexists; split.
+      specialize (Hx n); intuition; cleanup; try congruence.
     econstructor; eauto.
-    split; eauto.
   }
   { (** Write **)
-    intuition.
-    { (** bm1 h = None **)
-      specialize H1 with (1:= can_access_public pr) as Hx;
+    econstructor; eauto.
+    split_ors.
+    specialize H1 with (1:= can_access_public pr) as Hx;
       specialize (Hx h); intuition; cleanup; try congruence.
-      do 2 eexists; split.
-      econstructor; eauto.
-      split; eauto.
-    }
-    { (** d1 n = None **)
-      specialize H0 with (1:= can_access_public pr) as Hx;
+    specialize H0 with (1:= can_access_public pr) as Hx;
       specialize (Hx n); intuition; cleanup; try congruence.
-      do 2 eexists; split.
-      econstructor; eauto.
-      split; eauto.
-    }
   }
   { (** Unseal **)
-    specialize H1 with (1:= can_access_public pr) as Hx;
-    specialize (Hx h); intuition; cleanup; try congruence.
-    do 2 eexists; split.
     econstructor; eauto.
-    split; eauto.
+    split_ors.
+    specialize H1 with (1:= can_access_public pr) as Hx;
+      specialize (Hx h); intuition; cleanup; try congruence.
+    specialize H1 with (1:= can_access_public pr) as Hx;
+      specialize (Hx h); intuition; cleanup; try congruence.
+    right; eexists; split; eauto.
+    rewrite <- H6; eauto.
   }
   { (** Bind **)
-    intuition.
-    { (** p Failed **)
-      specialize IHp with (1:=H4)(2:=H1)(3:=H2)(4:=H3); cleanup.
-      do 2 eexists; split.
-      eapply FailBind; eauto.
-      eauto.
-    }
-    { (** p0 Failed **)
-      cleanup.
-      apply trace_secure_app_split in H3; cleanup.
-      eapply exec_equivalent_finished in H0; eauto; cleanup.
-      specialize H with (1:=H4)(2:=H6)(3:=H7)(4:=H3); cleanup.
-      do 2 eexists; split.
-      econstructor; eauto.
-      eauto.
-    }
+    split_ors; eauto.
+    econstructor; eauto.
+    
+    apply trace_secure_app_split in H3; cleanup.
+    eapply exec_equivalent_finished in H0; eauto.
+    cleanup; eauto.
+    eapply ExecBind; eauto.
   }
 Qed.
-
 
 Theorem exec_equivalent:
   forall T (p: prog T) pr tr d1 d2 bm1 bm2 hm (out: @result T),
     exec pr d1 bm1 hm p out tr ->
-    (forall tag, can_access pr tag -> equivalent_for tag d1 d2) ->
-    (forall tag, can_access pr tag -> blockmem_equivalent_for tag bm1 bm2) ->
+    (forall tag, can_access pr tag -> equivalent_for tag d1 d2 hm) ->
+    (forall tag, can_access pr tag -> blockmem_equivalent_for tag bm1 bm2 hm) ->
     trace_secure pr tr ->
     
     (exists d1' bm1' hm' (r: T), out = Finished d1' bm1' hm' r /\
      exists d2' bm2', exec pr d2 bm2 hm p (Finished d2' bm2' hm' r) tr /\
-    (forall tag, can_access pr tag -> equivalent_for tag d1' d2') /\
-    (forall tag, can_access pr tag -> blockmem_equivalent_for tag bm1' bm2')) \/
+    (forall tag, can_access pr tag -> equivalent_for tag d1' d2' hm') /\
+    (forall tag, can_access pr tag -> blockmem_equivalent_for tag bm1' bm2' hm')) \/
     
     (exists d1' bm1' hm', out = Crashed d1' bm1' hm' /\
      exists d2' bm2', exec pr d2 bm2 hm p (Crashed d2' bm2' hm') tr /\
-     (forall tag, can_access pr tag -> equivalent_for tag d1' d2') /\
-     (forall tag, can_access pr tag -> blockmem_equivalent_for tag bm1' bm2')) \/
+     (forall tag, can_access pr tag -> equivalent_for tag d1' d2' hm') /\
+     (forall tag, can_access pr tag -> blockmem_equivalent_for tag bm1' bm2' hm')) \/
     
-    (exists d1' bm1' hm', out = Failed d1' bm1' hm' /\
-     exists d2' bm2', exec pr d2 bm2 hm p (Failed d2' bm2' hm') tr /\
-     (forall tag, can_access pr tag -> equivalent_for tag d1' d2') /\
-     (forall tag, can_access pr tag -> blockmem_equivalent_for tag bm1' bm2')).
+    (exec pr d2 bm2 hm p Failed tr).
 Proof.
   intros.
   destruct out.
   left; do 4 eexists; split; eauto.
   eapply exec_equivalent_finished; eauto.
   right; left; do 3 eexists; split; eauto.
-  eapply exec_equivalent_crashed; eauto.
-  right; right; do 3 eexists; split; eauto.
-  eapply exec_equivalent_failed; eauto.
+  eapply exec_equivalent_crashed; eauto.  
+  right; right; eauto.
+  eapply exec_equivalent_failed; eauto.  
 Qed.
 
 
 Theorem exec_equivalent_rfinished:
   forall T T' (p1: prog T) (p2: prog T') pr tr d1 d2 bm1 bm2 hm d1' bm1' hm' (r: T),
     exec_recover pr d1 bm1 hm p1 p2 (RFinished T' d1' bm1' hm' r) tr ->
-    (forall tag, can_access pr tag -> equivalent_for tag d1 d2) ->
-    (forall tag, can_access pr tag -> blockmem_equivalent_for tag bm1 bm2) ->
+    (forall tag, can_access pr tag -> equivalent_for tag d1 d2 hm) ->
+    (forall tag, can_access pr tag -> blockmem_equivalent_for tag bm1 bm2 hm) ->
     trace_secure pr tr ->
     exists d2' bm2',
       exec_recover pr d2 bm2 hm p1 p2 (RFinished T' d2' bm2' hm' r) tr /\
-      (forall tag, can_access pr tag -> equivalent_for tag d1' d2') /\
-      (forall tag, can_access pr tag -> blockmem_equivalent_for tag bm1' bm2').
+      (forall tag, can_access pr tag -> equivalent_for tag d1' d2' hm') /\
+      (forall tag, can_access pr tag -> blockmem_equivalent_for tag bm1' bm2' hm').
 Proof.
   intros.
   inversion H; subst.
@@ -339,21 +410,17 @@ Proof.
 Qed.
 
 Theorem exec_equivalent_rfailed:
-  forall T T' (p1: prog T) (p2: prog T') pr tr d1 d2 bm1 bm2 hm d1' bm1' hm',
-    exec_recover pr d1 bm1 hm p1 p2 (RFailed T T' d1' bm1' hm') tr ->
-    (forall tag, can_access pr tag -> equivalent_for tag d1 d2) ->
-    (forall tag, can_access pr tag -> blockmem_equivalent_for tag bm1 bm2) ->
+  forall T T' (p1: prog T) (p2: prog T') pr tr d1 d2 bm1 bm2 hm,
+    exec_recover pr d1 bm1 hm p1 p2 (RFailed T T') tr ->
+    (forall tag, can_access pr tag -> equivalent_for tag d1 d2 hm) ->
+    (forall tag, can_access pr tag -> blockmem_equivalent_for tag bm1 bm2 hm) ->
     trace_secure pr tr ->
-    exists d2' bm2',
-      exec_recover pr d2 bm2 hm p1 p2 (RFailed T T' d2' bm2' hm') tr /\
-      (forall tag, can_access pr tag -> equivalent_for tag d1' d2') /\
-      (forall tag, can_access pr tag -> blockmem_equivalent_for tag bm1' bm2').
+    exec_recover pr d2 bm2 hm p1 p2 (RFailed T T') tr.
 Proof.
   intros.
   inversion H; subst.
-  eapply exec_equivalent_failed in H13; eauto; cleanup.
-  exists x, x0; split; eauto.
   econstructor; eauto.
+  eapply exec_equivalent_failed; eauto.  
 Qed.
 
 
@@ -363,23 +430,20 @@ Theorem exec_equivalent_recover:
     exec_recover pr d1 bm1 hm p1 p2 out tr ->
     trace_secure pr tr ->
     forall d2 bm2,
-    (forall tag, can_access pr tag -> equivalent_for tag d1 d2) ->
-    (forall tag, can_access pr tag -> blockmem_equivalent_for tag bm1 bm2) ->
+    (forall tag, can_access pr tag -> equivalent_for tag d1 d2 hm) ->
+    (forall tag, can_access pr tag -> blockmem_equivalent_for tag bm1 bm2 hm) ->
     
     (exists d1' bm1' hm' r, out = RFinished T' d1' bm1' hm' r /\
      exists d2' bm2', exec_recover pr d2 bm2 hm p1 p2 (RFinished T' d2' bm2' hm' r) tr /\
-    (forall tag, can_access pr tag -> equivalent_for tag d1' d2') /\
-    (forall tag, can_access pr tag -> blockmem_equivalent_for tag bm1' bm2')) \/
+    (forall tag, can_access pr tag -> equivalent_for tag d1' d2' hm') /\
+    (forall tag, can_access pr tag -> blockmem_equivalent_for tag bm1' bm2' hm')) \/
 
-    (exists d1' bm1' hm', out = RFailed T T' d1' bm1' hm' /\
-     exists d2' bm2', exec_recover pr d2 bm2 hm p1 p2 (RFailed T T' d2' bm2' hm') tr /\
-    (forall tag, can_access pr tag -> equivalent_for tag d1' d2') /\
-    (forall tag, can_access pr tag -> blockmem_equivalent_for tag bm1' bm2')) \/
+    (out = RFailed T T' /\ exec_recover pr d2 bm2 hm p1 p2 (RFailed T T') tr) \/
     
     (exists d1' bm1' hm' r, out = RRecovered T d1' bm1' hm' r /\
      exists d2' bm2', exec_recover pr d2 bm2 hm p1 p2 (RRecovered T d2' bm2' hm' r) tr /\
-    (forall tag, can_access pr tag -> equivalent_for tag d1' d2') /\
-    (forall tag, can_access pr tag -> blockmem_equivalent_for tag bm1' bm2')).
+    (forall tag, can_access pr tag -> equivalent_for tag d1' d2' hm') /\
+    (forall tag, can_access pr tag -> blockmem_equivalent_for tag bm1' bm2' hm')).
 Proof.
   induction 1; intros.
   { (** p1 Finished **)
@@ -387,29 +451,44 @@ Proof.
     eapply exec_equivalent_rfinished; eauto.
     econstructor; eauto.
   }
-  { (** p1 Finished **)
-    right; left; do 3 eexists; split; eauto.
+  { (** p1 Failed **)
+    right; left; split; eauto.
     eapply exec_equivalent_rfailed; eauto.
     econstructor; eauto.
   }
   { (** p1 Crashed then p2 Finished **)
     clear IHexec_recover.
-    inversion H1; subst; clear H1.
     apply trace_secure_app_split in H2; cleanup.
     eapply exec_equivalent_crashed in H; eauto; cleanup.
-    eapply possible_crash_equivalent in H5 as Hx; eauto; cleanup.
-    eapply exec_equivalent_finished in H16 as Hp2; eauto; cleanup.
+    eapply possible_crash_equivalent in H6 as Hx; eauto; cleanup.
+    eapply exec_equivalent_rfinished in H1; eauto; cleanup.
+    (* eapply exec_equivalent_finished in H16 as Hp2; eauto; cleanup. *)
     right; right; do 4 eexists; split; eauto.
     do 2 eexists; split; eauto.
     econstructor; eauto.
-    econstructor; eauto.
+    - intros; unfold blockmem_equivalent_for in *; intros.
+      unfold empty_mem; simpl; eauto.
   }
   { (** p1 Crashed then p2 Crashed **)
     right; right; do 4 eexists; split; eauto.
     apply trace_secure_app_split in H2; cleanup.
     eapply exec_equivalent_crashed in H; eauto; cleanup.
     eapply possible_crash_equivalent in H6 as Hx; eauto; cleanup.
-    specialize IHexec_recover with (1:=H2)(2:=H9)(3:=H7).
+    specialize IHexec_recover with (1:=H2).
+    edestruct IHexec_recover.
+    {
+      intros; unfold equivalent_for in *; intros.
+      specialize (H9 _ H10).
+      specialize (H9 a); split_ors; eauto.
+      right; do 2 eexists; intuition eauto.
+    }
+    {
+      eassign (@empty_mem handle handle_eq_dec tagged_block).
+      intros; unfold blockmem_equivalent_for in *; intros.
+      unfold empty_mem; simpl; eauto.
+    }
+   
+    all: cleanup; try congruence.
     intuition; cleanup; try congruence.
     inversion H10; subst; clear H10.
     do 2 eexists; split; eauto.
@@ -421,26 +500,26 @@ Qed.
   Lemma exec_equivalent_for_viewer_finished:
   forall T (p: prog T) caller viewer d d' bm bm' hm d1 bm1 hm1 r1 tr,
     exec caller d bm hm p (Finished d1 bm1 hm1 r1) tr ->
-    (forall tag, can_access viewer tag -> equivalent_for tag d d') ->
-    (forall tag, can_access viewer tag -> blockmem_equivalent_for tag bm bm') ->
+    (forall tag, can_access viewer tag -> equivalent_for tag d d' hm) ->
+    (forall tag, can_access viewer tag -> blockmem_equivalent_for tag bm bm' hm) ->
     only_public_operations tr ->
     exists d2 bm2 tr2,
       exec caller d' bm' hm p (Finished d2 bm2 hm1 r1) tr2 /\
-      (forall tag, can_access viewer tag -> equivalent_for tag d1 d2) /\
-      (forall tag, can_access viewer tag -> blockmem_equivalent_for tag bm1 bm2).
+      (forall tag, can_access viewer tag -> equivalent_for tag d1 d2 hm1) /\
+      (forall tag, can_access viewer tag -> blockmem_equivalent_for tag bm1 bm2 hm1).
   Proof.
      induction p; intros;  
   inv_exec_perm; cleanup; simpl in *;
   try solve [repeat eexists; [econstructor; eauto|eauto|eauto] ].
   { (** Read **)
-    destruct tb.
+    destruct bs.
     specialize H1 with (1:= can_access_public viewer) as Hx;
     specialize (Hx r1); intuition; cleanup; try congruence.
     specialize H0 with (1:= can_access_public viewer) as Hx;
     specialize (Hx n); intuition; cleanup; try congruence.
     destruct x0, t0.
     unfold vsmerge in *; simpl in *.
-    inversion H5; inversion H6; simpl in *; subst.
+    repeat (denote (Forall2 _ (_::_)(_::_)) as Hf; inversion Hf; clear Hf; subst).
     do 3 eexists; split.
     econstructor; eauto.
     split; eauto.
@@ -453,17 +532,18 @@ Qed.
     split; eauto.
     split; eauto.
     intros.
-    simpl in *; eauto.    
+    simpl in *; eauto.
     specialize H0 with (1:= H) as Hx;
     specialize (Hx n); intuition; cleanup; try congruence.
     unfold vsmerge in *; simpl in *.
-    inversion H10; inversion H12; simpl in *; subst.
+    repeat (denote (Forall2 _ (_::_)(_::_)) as Hf; inversion Hf; clear Hf; subst).
     eauto.
     repeat rewrite Mem.upd_ne; eauto.
     eapply H1; eauto.
   }
   { (** Write **)
-    destruct tb, tbs, t0.
+    destruct b, bs, t; simpl in *.
+    destruct (hm1 n0) eqn: D.    
     destruct (can_access_dec viewer t).
     { (** can access **)
       specialize H0 with (1:= can_access_public viewer) as Hx;
@@ -499,7 +579,7 @@ Qed.
       econstructor; eauto.
       split; eauto.
       unfold equivalent_for; intros.
-      destruct (tag_dec t2 tag); subst; intuition.
+      destruct (tag_dec t tag); subst; intuition.
       specialize H0 with (1:= H) as Hx;
       specialize (Hx n); destruct Hx; cleanup; try congruence.
       destruct (addr_eq_dec a n); subst.
@@ -512,7 +592,34 @@ Qed.
       unfold vsmerge in *; simpl in *; eauto.
       unfold vsmerge in *; simpl in *; eauto.
       econstructor.
-      simpl; intros; intuition.
+      simpl; intros; cleanup; intuition.
+      eauto.
+      repeat rewrite Mem.upd_ne; eauto.
+      eapply H0; eauto.
+    }
+    { (** inconsistent **)
+      specialize H0 with (1:= can_access_public viewer) as Hx;
+      specialize (Hx n); intuition; cleanup; try congruence.
+      specialize H1 with (1:= can_access_public viewer) as Hx;
+      specialize (Hx h); intuition; cleanup; try congruence.
+      destruct x0, x1; simpl in *; cleanup.
+      do 3 eexists; split.
+      econstructor; eauto.
+      split; eauto.
+      unfold equivalent_for; intros.
+      specialize H0 with (1:= H) as Hx;
+      specialize (Hx n); destruct Hx; cleanup; try congruence.
+      destruct (addr_eq_dec a n); subst.
+      right.
+      repeat rewrite Mem.upd_eq; eauto.
+      do 2 eexists; eauto.
+      split; eauto.
+      split; eauto.
+      split.
+      unfold vsmerge in *; simpl in *; eauto.
+      unfold vsmerge in *; simpl in *; eauto.
+      econstructor.
+      simpl; intros; congruence.
       eauto.
       repeat rewrite Mem.upd_ne; eauto.
       eapply H0; eauto.
@@ -534,7 +641,7 @@ Qed.
   }
   { (** Unseal **)
     intuition.
-    destruct tb; simpl in *.
+    destruct b; simpl in *.
     specialize H1 with (1:= can_access_public viewer) as Hx;
     specialize (Hx h); intuition; cleanup; try congruence.
     simpl in *; intuition; subst.
@@ -548,15 +655,78 @@ Qed.
     specialize H0 with (1:= H) as Hx.
     unfold sync_mem.
     specialize (Hx a); intuition; cleanup; eauto.
-    rewrite H4, H5; eauto.
-    rewrite H3, H4; eauto.
+    repeat match goal with
+           | [H: ?x = _ |- context [?x] ] => rewrite H
+           end; eauto.
+    repeat match goal with
+           | [H: ?x = _ |- context [?x] ] => rewrite H
+           end; eauto.
     destruct x, x0.
-    right; repeat eexists; eauto.
     unfold vsmerge in *; simpl in *; eauto.
-    inversion H5; subst.
-    econstructor; eauto.
-    unfold vsmerge in *; simpl in *; eauto.
-    inversion H6; subst; auto.
+    repeat (denote (Forall2 _ (_::_)(_::_)) as Hf; inversion Hf; clear Hf; subst).
+    right; repeat eexists; simpl; eauto.    
+  }
+  { (** ChDom **)
+    cleanup.
+    specialize H0 with (1:= can_access_public viewer) as Hdt'.
+    specialize H1 with (1:= can_access_public viewer) as Hbt'.
+    repeat eexists; [econstructor; eauto| |eauto].
+    {
+      unfold equivalent_for in *; intros.
+      specialize (Hdt' a); intuition; cleanup; eauto.
+      specialize H0 with (1:= H) as Hx.
+      specialize (Hx a); intuition; cleanup; eauto.
+      repeat match goal with
+             | [H: ?x = _ |- context [?x] ] => rewrite H
+             end; eauto.
+      destruct x1, x2.
+      right; repeat eexists; eauto.
+      unfold vsmerge in *; simpl in *; eauto.
+      repeat (denote (Forall2 _ (_::_)(_::_)) as Hf; inversion Hf; clear Hf; subst).
+      destruct (addr_eq_dec n (fst t0)); subst.
+      - econstructor; eauto.
+        eapply forall_forall2.
+        rewrite Forall_forall; intros.
+        destruct (addr_eq_dec (fst t0) (fst (fst x))); subst.
+        + cleanup.
+          rewrite Mem.upd_eq in H6; eauto.
+          cleanup.
+          eapply forall2_forall in H16; rewrite Forall_forall in H16; eauto.
+          eapply H16; eauto.
+          setoid_rewrite <- H10; eauto.
+        + rewrite Mem.upd_ne in H6; eauto.
+          cleanup.
+          eapply forall2_forall in H13; rewrite Forall_forall in H13; eauto.
+        + eapply forall2_length; eauto.
+      - cleanup.
+        econstructor; eauto.
+        rewrite Mem.upd_ne; eauto.
+        eapply forall_forall2.
+        rewrite Forall_forall; intros.
+        destruct (addr_eq_dec n (fst (fst x))); subst.
+        + rewrite Mem.upd_eq in H6; eauto.
+          cleanup.
+          eapply forall2_forall in H16; rewrite Forall_forall in H16; eauto.
+        + rewrite Mem.upd_ne in H6; eauto.
+          cleanup.
+          eapply forall2_forall in H13; rewrite Forall_forall in H13; eauto.
+        + eapply forall2_length; eauto.
+    }
+    {
+      unfold blockmem_equivalent_for in *; intros.
+      specialize (Hbt' a); intuition; cleanup; eauto.
+      specialize H1 with (1:= H) as Hx.
+      specialize (Hx a); intuition; cleanup; eauto.
+      repeat match goal with
+             | [H: ?x = _ |- context [?x] ] => rewrite H
+             end; eauto.
+      destruct x1, x2.
+      right; repeat eexists; eauto.
+      simpl in *; eauto.
+      destruct (addr_eq_dec n n0); subst.
+      rewrite Mem.upd_eq; eauto.
+      rewrite Mem.upd_ne; eauto.
+    }
   }
   { (** Bind **)
     apply only_public_operations_app in H3; cleanup.
@@ -564,18 +734,21 @@ Qed.
     specialize H with (1:=H4)(2:=H7)(3:=H8)(4:=H3); cleanup.
     repeat eexists; [econstructor; eauto| |]; eauto.
   }
-  Qed.
+
+  Unshelve.
+  all: try exact addr; eauto.
+  all: try exact nil.
+  all: try exact eq.
+Qed.
+
 
   Lemma exec_equivalent_for_viewer_failed:
-  forall T (p: prog T) caller viewer d d' bm bm' hm d1 bm1 hm1 tr,
-    exec caller d bm hm p (Failed d1 bm1 hm1) tr ->
-    (forall tag, can_access viewer tag -> equivalent_for tag d d') ->
-    (forall tag, can_access viewer tag -> blockmem_equivalent_for tag bm bm') ->
+  forall T (p: prog T) caller viewer d d' bm bm' hm tr,
+    exec caller d bm hm p Failed tr ->
+    (forall tag, can_access viewer tag -> equivalent_for tag d d' hm) ->
+    (forall tag, can_access viewer tag -> blockmem_equivalent_for tag bm bm' hm) ->
     only_public_operations tr ->
-    exists d2 bm2 tr2,
-      exec caller d' bm' hm p (Failed d2 bm2 hm1) tr2 /\
-      (forall tag, can_access viewer tag -> equivalent_for tag d1 d2) /\
-      (forall tag, can_access viewer tag -> blockmem_equivalent_for tag bm1 bm2).
+    exists tr2, exec caller d' bm' hm p Failed tr2.
   Proof.
   induction p; intros;  
   inv_exec_perm; cleanup; simpl in *;
@@ -583,50 +756,48 @@ Qed.
   { (** Read **)
     specialize H0 with (1:= can_access_public viewer) as Hx;
     specialize (Hx n); intuition; cleanup; try congruence.
-    do 3 eexists; split.
-    econstructor; eauto.
-    split; eauto.
+    eexists; econstructor; eauto.
   }
   { (** Write **)
     intuition.
     { (** bm1 h = None **)
       specialize H1 with (1:= can_access_public viewer) as Hx;
       specialize (Hx h); intuition; cleanup; try congruence.
-      do 3 eexists; split.
-      econstructor; eauto.
-      split; eauto.
+      eexists; econstructor; eauto.
     }
     { (** d1 n = None **)
       specialize H0 with (1:= can_access_public viewer) as Hx;
       specialize (Hx n); intuition; cleanup; try congruence.
-      do 3 eexists; split.
-      econstructor; eauto.
-      split; eauto.
+      eexists; econstructor; eauto.
     }
   }
   { (** Unseal **)
+    eexists; econstructor; eauto.
+    split_ors.
     specialize H1 with (1:= can_access_public viewer) as Hx;
     specialize (Hx h); intuition; cleanup; try congruence.
-    do 3 eexists; split.
-    econstructor; eauto.
-    split; eauto.
+    
+    specialize H1 with (1:= can_access_public viewer) as Hx;
+      specialize (Hx h); intuition; cleanup; try congruence.
+    right; eexists; econstructor; eauto.
+    rewrite <- H6; eauto.
+  }
+  { (** ChDom **)
+    eexists; econstructor; eauto.
   }
   { (** Bind **)
     intuition.
     { (** p Failed **)
       specialize IHp with (1:=H4)(2:=H1)(3:=H2)(4:=H3); cleanup.
-      do 3 eexists; split.
+      eexists.
       eapply FailBind; eauto.
-      eauto.
     }
     { (** p0 Failed **)
       cleanup.
       apply only_public_operations_app in H3; cleanup.
       eapply exec_equivalent_for_viewer_finished in H0; eauto; cleanup.
       specialize H with (1:=H4)(2:=H6)(3:=H7)(4:=H3); cleanup.
-      do 3 eexists; split.
-      econstructor; eauto.
-      eauto.
+      eexists; econstructor; eauto.
     }
   }
   Qed.
@@ -634,13 +805,13 @@ Qed.
   Lemma exec_equivalent_for_viewer_crashed:
   forall T (p: prog T) caller viewer d d' bm bm' hm d1 bm1 hm1 tr,
     exec caller d bm hm p (Crashed d1 bm1 hm1) tr ->
-    (forall tag, can_access viewer tag -> equivalent_for tag d d') ->
-    (forall tag, can_access viewer tag -> blockmem_equivalent_for tag bm bm') ->
+    (forall tag, can_access viewer tag -> equivalent_for tag d d' hm) ->
+    (forall tag, can_access viewer tag -> blockmem_equivalent_for tag bm bm' hm) ->
     only_public_operations tr ->
     exists d2 bm2 tr2,
       exec caller d' bm' hm p (Crashed d2 bm2 hm1) tr2 /\
-      (forall tag, can_access viewer tag -> equivalent_for tag d1 d2) /\
-      (forall tag, can_access viewer tag -> blockmem_equivalent_for tag bm1 bm2).
+      (forall tag, can_access viewer tag -> equivalent_for tag d1 d2 hm1) /\
+      (forall tag, can_access viewer tag -> blockmem_equivalent_for tag bm1 bm2 hm1).
   Proof.
   induction p; intros;  
   inv_exec_perm; cleanup; simpl in *;
@@ -669,23 +840,21 @@ Qed.
 Lemma exec_equivalent_for_viewer:
   forall T (p: prog T) caller viewer d d' bm bm' hm res tr,
     exec caller d bm hm p res tr ->
-    (forall tag, can_access viewer tag -> equivalent_for tag d d') ->
-    (forall tag, can_access viewer tag -> blockmem_equivalent_for tag bm bm') ->
+    (forall tag, can_access viewer tag -> equivalent_for tag d d' hm) ->
+    (forall tag, can_access viewer tag -> blockmem_equivalent_for tag bm bm' hm) ->
     only_public_operations tr ->
      (exists d1 bm1 hm1 r1, res = Finished d1 bm1 hm1 r1 /\ 
       exists d2 bm2 tr2, exec caller d' bm' hm p (Finished d2 bm2 hm1 r1) tr2 /\
-      (forall tag, can_access viewer tag -> equivalent_for tag d1 d2) /\
-      (forall tag, can_access viewer tag -> blockmem_equivalent_for tag bm1 bm2)) \/
+      (forall tag, can_access viewer tag -> equivalent_for tag d1 d2 hm1) /\
+      (forall tag, can_access viewer tag -> blockmem_equivalent_for tag bm1 bm2 hm1)) \/
       
       (exists d1 bm1 hm1, res = Crashed d1 bm1 hm1 /\
        exists d2 bm2 tr2, exec caller d' bm' hm p (Crashed d2 bm2 hm1) tr2 /\
-      (forall tag, can_access viewer tag -> equivalent_for tag d1 d2) /\
-      (forall tag, can_access viewer tag -> blockmem_equivalent_for tag bm1 bm2)) \/
+      (forall tag, can_access viewer tag -> equivalent_for tag d1 d2 hm1) /\
+      (forall tag, can_access viewer tag -> blockmem_equivalent_for tag bm1 bm2 hm1)) \/
       
-      (exists d1 bm1 hm1, res = Failed d1 bm1 hm1 /\
-       exists d2 bm2 tr2, exec caller d' bm' hm p (Failed d2 bm2 hm1) tr2 /\
-      (forall tag, can_access viewer tag -> equivalent_for tag d1 d2) /\
-      (forall tag, can_access viewer tag -> blockmem_equivalent_for tag bm1 bm2)).
+      (res = Failed /\
+       exists tr2, exec caller d' bm' hm p Failed tr2).
 Proof.
   intros.
   destruct res.
@@ -693,6 +862,6 @@ Proof.
   eapply exec_equivalent_for_viewer_finished; eauto.
   right; left; do 3 eexists; split; eauto.
   eapply exec_equivalent_for_viewer_crashed; eauto.
-  right; right; do 3 eexists; split; eauto.
+  right; right; split; eauto.
   eapply exec_equivalent_for_viewer_failed; eauto.
 Qed.
